make nondet safe again

src/cbor/pulse/raw/CBOR.Pulse.API.Nondet.C.fst
@@ -17,33 +17,29 @@ let cbor_nondet_serialize () = cbor_nondet_serialize_to_arrayptr (Rust.cbor_nond
 
 let cbor_nondet_major_type () x #p #y = Rust.cbor_nondet_major_type () x #p #y
 
-let cbor_nondet_read_simple_value () x #p #y = Rust.cbor_nondet_read_simple_value () x #p #y
+let cbor_nondet_read_simple_value () = read_simple_value_safe (cbor_nondet_major_type ()) (Rust.cbor_nondet_read_simple_value ())
 
 let cbor_nondet_elim_simple () = Rust.cbor_nondet_elim_simple ()
 
-let cbor_nondet_read_uint64 () x #p #y = Rust.cbor_nondet_read_uint64 () x #p #y
+let cbor_nondet_read_uint64 () = read_uint64_safe (cbor_nondet_major_type ()) (Rust.cbor_nondet_read_uint64 ())
 
 let cbor_nondet_elim_int64 () = Rust.cbor_nondet_elim_int64 ()
 
-let cbor_nondet_get_string_length () x #p #y = Rust.cbor_nondet_get_string_length () x #p #y
+let cbor_nondet_get_string () = get_string_as_arrayptr_safe (cbor_nondet_major_type ()) (Rust.cbor_nondet_get_string_length ()) (get_string_as_arrayptr (Rust.cbor_nondet_get_string ()))
 
-let cbor_nondet_get_string () = get_string_as_arrayptr (Rust.cbor_nondet_get_string ())
+let cbor_nondet_get_tagged () = get_tagged_safe (cbor_nondet_major_type ()) (Rust.cbor_nondet_get_tagged_tag ()) (Rust.cbor_nondet_get_tagged_payload ())
 
-let cbor_nondet_get_tagged_tag () x #p #y = Rust.cbor_nondet_get_tagged_tag () x #p #y
-
-let cbor_nondet_get_tagged_payload () x #p #y = Rust.cbor_nondet_get_tagged_payload () x #p #y
-
-let cbor_nondet_get_array_length () x #p #y = Rust.cbor_nondet_get_array_length () x #p #y
+let cbor_nondet_get_array_length () = get_array_length_safe (cbor_nondet_major_type ()) (Rust.cbor_nondet_get_array_length ())
 
 let cbor_nondet_array_iterator_match = Rust.cbor_nondet_array_iterator_match
 
-let cbor_nondet_array_iterator_start () x #p #y = Rust.cbor_nondet_array_iterator_start () x #p #y
+let cbor_nondet_array_iterator_start () = array_iterator_start_safe (cbor_nondet_major_type ()) (Rust.cbor_nondet_array_iterator_start ())
 
 let cbor_nondet_array_iterator_is_empty () x #p #y = Rust.cbor_nondet_array_iterator_is_empty () x #p #y
 
 let cbor_nondet_array_iterator_length () x #p #y = Rust.cbor_nondet_array_iterator_length () x #p #y
 
-let cbor_nondet_array_iterator_next () x #y #py #z = Rust.cbor_nondet_array_iterator_next () x #y #py #z
+let cbor_nondet_array_iterator_next () = array_iterator_next_safe (cbor_nondet_array_iterator_is_empty ()) (Rust.cbor_nondet_array_iterator_next ())
 
 let cbor_nondet_array_iterator_truncate () x len #p #y = Rust.cbor_nondet_array_iterator_truncate () x len #p #y
 
@@ -51,27 +47,27 @@ let cbor_nondet_array_iterator_share () = Rust.cbor_nondet_array_iterator_share 
 
 let cbor_nondet_array_iterator_gather () = Rust.cbor_nondet_array_iterator_gather ()
 
-let cbor_nondet_get_array_item () x i #p #y = Rust.cbor_nondet_get_array_item () x i #p #y
+let cbor_nondet_get_array_item () = get_array_item_safe (cbor_nondet_major_type ()) (Rust.cbor_nondet_get_array_length ()) (Rust.cbor_nondet_get_array_item ())
 
-let cbor_nondet_get_map_length () x #p #y = Rust.cbor_nondet_get_map_length () x #p #y
+let cbor_nondet_get_map_length () = get_map_length_safe (cbor_nondet_major_type ()) (Rust.cbor_nondet_get_map_length ())
 
 let cbor_nondet_map_iterator_match = Rust.cbor_nondet_map_iterator_match
 
-let cbor_nondet_map_iterator_start () x #p #y = Rust.cbor_nondet_map_iterator_start () x #p #y
+let cbor_nondet_map_iterator_start () = map_iterator_start_safe (cbor_nondet_major_type ()) (Rust.cbor_nondet_map_iterator_start ())
 
 let cbor_nondet_map_iterator_is_empty () x #p #y = Rust.cbor_nondet_map_iterator_is_empty () x #p #y
 
 let cbor_nondet_map_entry_match = Rust.cbor_nondet_map_entry_match
 
-let cbor_nondet_map_iterator_next () x #y #py #z = Rust.cbor_nondet_map_iterator_next () x #y #py #z
+let cbor_nondet_map_entry_key () x #p #y = Rust.cbor_nondet_map_entry_key () x #p #y
+
+let cbor_nondet_map_entry_value () x #p #y = Rust.cbor_nondet_map_entry_value () x #p #y
+
+let cbor_nondet_map_iterator_next () = map_iterator_next_safe (cbor_nondet_map_iterator_is_empty ()) (Rust.cbor_nondet_map_iterator_next ()) (Rust.cbor_nondet_map_entry_share ()) (Rust.cbor_nondet_map_entry_gather ()) (cbor_nondet_map_entry_key ()) (cbor_nondet_map_entry_value ())
 
 let cbor_nondet_map_iterator_share () = Rust.cbor_nondet_map_iterator_share ()
 
 let cbor_nondet_map_iterator_gather () = Rust.cbor_nondet_map_iterator_gather ()
-
-let cbor_nondet_map_entry_key () x #p #y = Rust.cbor_nondet_map_entry_key () x #p #y
-
-let cbor_nondet_map_entry_value () x #p #y = Rust.cbor_nondet_map_entry_value () x #p #y
 
 let cbor_nondet_map_entry_share () = Rust.cbor_nondet_map_entry_share ()
 
@@ -79,24 +75,22 @@ let cbor_nondet_map_entry_gather () = Rust.cbor_nondet_map_entry_gather ()
 
 let cbor_nondet_equal x1 #p1 #v1 x2 #p2 #v2 = Rust.cbor_nondet_equal x1 #p1 #v1 x2 #p2 #v2
 
-fn cbor_nondet_map_get (_: unit) : map_get_by_ref_t #_ cbor_nondet_match =
-  (x: _) (k: _) (dest: _) (#px: _) (#vx: _) (#pk: _) (#vk: _) (#vdest0: _)
-{
-  Rust.cbor_nondet_map_get () x k dest
-}
+let cbor_nondet_map_get () = map_get_by_ref_safe (cbor_nondet_major_type ()) (Rust.cbor_nondet_map_get ())
 
-let cbor_nondet_mk_simple_value () v = Rust.cbor_nondet_mk_simple_value () v
+let cbor_nondet_mk_simple_value () = mk_simple_safe (Rust.cbor_nondet_mk_simple_value ())
 
-let cbor_nondet_mk_int64 () ty v = Rust.cbor_nondet_mk_int64 () ty v
+let cbor_nondet_mk_uint64 () v = Rust.cbor_nondet_mk_int64 () cbor_major_type_uint64 v
+
+let cbor_nondet_mk_neg_int64 () v = Rust.cbor_nondet_mk_int64 () cbor_major_type_neg_int64 v
 
 let cbor_nondet_mk_byte_string () = mk_string_from_arrayptr (Rust.cbor_nondet_mk_string ()) cbor_major_type_byte_string
 
 let cbor_nondet_mk_text_string () = mk_string_from_arrayptr (Rust.cbor_nondet_mk_string ()) cbor_major_type_text_string
 
-let cbor_nondet_mk_tagged () tag r #pr #v #pv #v' = Rust.cbor_nondet_mk_tagged () tag r #pr #v #pv #v'
+let cbor_nondet_mk_tagged () = mk_tagged_safe (Rust.cbor_nondet_mk_tagged ())
 
 let cbor_nondet_mk_array () = mk_array_from_arrayptr (Rust.cbor_nondet_mk_array ())
 
 let cbor_nondet_mk_map_entry () xk xv #pk #vk #pv #vv = Rust.cbor_nondet_mk_map_entry () xk xv #pk #vk #pv #vv
 
-let cbor_nondet_mk_map_gen () = cbor_mk_map_from_arrayptr_safe (Rust.cbor_nondet_mk_map_gen ())
+let cbor_nondet_mk_map () = cbor_mk_map_from_arrayptr_safe (Rust.cbor_nondet_mk_map_gen ())
