src/cbor/pulse/CBOR.Pulse.API.Nondet.C.fsti
@@ -33,33 +33,29 @@ val cbor_nondet_serialize
 
 val cbor_nondet_major_type (_: unit) : get_major_type_t u#0 #_ cbor_nondet_match
 
-val cbor_nondet_read_simple_value (_: unit) : read_simple_value_t u#0 #_ cbor_nondet_match
+val cbor_nondet_read_simple_value (_: unit) : read_simple_value_safe_t u#0 #_ cbor_nondet_match
 
 val cbor_nondet_elim_simple (_: unit) : elim_simple_t u#0 #_ cbor_nondet_match
 
-val cbor_nondet_read_uint64 (_: unit) : read_uint64_t u#0 #_ cbor_nondet_match
+val cbor_nondet_read_uint64 (_: unit) : read_uint64_safe_t u#0 #_ cbor_nondet_match
 
 val cbor_nondet_elim_int64 (_: unit) : elim_int64_t u#0 #_ cbor_nondet_match
 
-val cbor_nondet_get_string_length (_: unit) : get_string_length_t u#0 #_ cbor_nondet_match
+val cbor_nondet_get_string (_: unit) : get_string_as_arrayptr_safe_t u#0 #_ cbor_nondet_match
 
-val cbor_nondet_get_string (_: unit) : get_string_as_arrayptr_t u#0 #_ cbor_nondet_match
+val cbor_nondet_get_tagged (_: unit) : get_tagged_safe_t #_ cbor_nondet_match
 
-val cbor_nondet_get_tagged_tag (_: unit) : get_tagged_tag_t u#0 #_ cbor_nondet_match
-
-val cbor_nondet_get_tagged_payload (_: unit) : get_tagged_payload_t u#0 #_ cbor_nondet_match
-
-val cbor_nondet_get_array_length (_: unit) : get_array_length_t u#0 #_ cbor_nondet_match
+val cbor_nondet_get_array_length (_: unit) : get_array_length_safe_t u#0 #_ cbor_nondet_match
 
 val cbor_nondet_array_iterator_match: perm -> cbor_nondet_array_iterator_t -> list Spec.cbor -> slprop
 
-val cbor_nondet_array_iterator_start (_: unit) : array_iterator_start_t u#0 u#0 #_ #_ cbor_nondet_match cbor_nondet_array_iterator_match
+val cbor_nondet_array_iterator_start (_: unit) : array_iterator_start_safe_t u#0 #_ #_ cbor_nondet_match cbor_nondet_array_iterator_match
 
 val cbor_nondet_array_iterator_is_empty (_: unit) : array_iterator_is_empty_t u#0 #_ cbor_nondet_array_iterator_match
 
 val cbor_nondet_array_iterator_length (_: unit) : array_iterator_length_t u#0 #_ cbor_nondet_array_iterator_match
 
-val cbor_nondet_array_iterator_next (_: unit) : array_iterator_next_t u#0 #_ #_ cbor_nondet_match cbor_nondet_array_iterator_match
+val cbor_nondet_array_iterator_next (_: unit) : array_iterator_next_safe_t #_ #_ cbor_nondet_match cbor_nondet_array_iterator_match
 
 val cbor_nondet_array_iterator_truncate (_: unit) : array_iterator_truncate_t u#0 #_ cbor_nondet_array_iterator_match
 
@@ -67,27 +63,27 @@ val cbor_nondet_array_iterator_share (_: unit) : share_t u#0 u#0 #_ #_ cbor_nond
 
 val cbor_nondet_array_iterator_gather (_: unit) : gather_t u#0 u#0 #_ #_ cbor_nondet_array_iterator_match
 
-val cbor_nondet_get_array_item (_: unit) : get_array_item_t u#0 #_ cbor_nondet_match
+val cbor_nondet_get_array_item (_: unit) : get_array_item_safe_t #_ cbor_nondet_match
 
-val cbor_nondet_get_map_length (_: unit) : get_map_length_t u#0 #_ cbor_nondet_match
+val cbor_nondet_get_map_length (_: unit) : get_map_length_safe_t u#0 #_ cbor_nondet_match
 
 val cbor_nondet_map_iterator_match: perm -> cbor_nondet_map_iterator_t -> list (Spec.cbor & Spec.cbor) -> slprop
 
-val cbor_nondet_map_iterator_start (_: unit) : map_iterator_start_t u#0 u#0 #_ #_ cbor_nondet_match cbor_nondet_map_iterator_match
+val cbor_nondet_map_iterator_start (_: unit) : map_iterator_start_safe_t u#0 #_ #_ cbor_nondet_match cbor_nondet_map_iterator_match
 
 val cbor_nondet_map_iterator_is_empty (_: unit) : map_iterator_is_empty_t u#0 #_ cbor_nondet_map_iterator_match
 
 val cbor_nondet_map_entry_match: perm -> cbor_nondet_map_entry_t -> Spec.cbor & Spec.cbor -> slprop
 
-val cbor_nondet_map_iterator_next (_: unit) : map_iterator_next_t u#0 #_ #_ cbor_nondet_map_entry_match cbor_nondet_map_iterator_match
+val cbor_nondet_map_entry_key (_: unit) : map_entry_key_t u#0 u#0 #_ #_ cbor_nondet_map_entry_match cbor_nondet_match
+
+val cbor_nondet_map_entry_value (_: unit) : map_entry_value_t u#0 u#0 #_ #_ cbor_nondet_map_entry_match cbor_nondet_match
+
+val cbor_nondet_map_iterator_next (_: unit) : map_iterator_next_safe_t #_ #_ cbor_nondet_match cbor_nondet_map_iterator_match
 
 val cbor_nondet_map_iterator_share (_: unit) : share_t u#0 u#0 #_ #_ cbor_nondet_map_iterator_match
 
 val cbor_nondet_map_iterator_gather (_: unit) : gather_t u#0 u#0 #_ #_ cbor_nondet_map_iterator_match
-
-val cbor_nondet_map_entry_key (_: unit) : map_entry_key_t u#0 u#0 #_ #_ cbor_nondet_map_entry_match cbor_nondet_match
-
-val cbor_nondet_map_entry_value (_: unit) : map_entry_value_t u#0 u#0 #_ #_ cbor_nondet_map_entry_match cbor_nondet_match
 
 val cbor_nondet_map_entry_share
   (_: unit)
@@ -118,23 +114,25 @@ val cbor_nondet_equal
 )
 
 val cbor_nondet_map_get (_: unit)
-: map_get_by_ref_t #_ cbor_nondet_match
+: map_get_by_ref_safe_t #_ cbor_nondet_match
 
 (* Constructors *)
 
-val cbor_nondet_mk_simple_value (_: unit) : mk_simple_t u#0 #_ cbor_nondet_match
+val cbor_nondet_mk_simple_value (_: unit) : mk_simple_safe_t #_ cbor_nondet_match
 
-val cbor_nondet_mk_int64 (_: unit) : mk_int64_t u#0 #_ cbor_nondet_match
+val cbor_nondet_mk_uint64 (_: unit) : mk_int64_gen_t u#0 #_ cbor_nondet_match cbor_major_type_uint64
+
+val cbor_nondet_mk_neg_int64 (_: unit) : mk_int64_gen_t u#0 #_ cbor_nondet_match cbor_major_type_neg_int64
 
 val cbor_nondet_mk_byte_string (_: unit) : mk_string_from_arrayptr_t #_ cbor_nondet_match cbor_major_type_byte_string
 
 val cbor_nondet_mk_text_string (_: unit) : mk_string_from_arrayptr_t #_ cbor_nondet_match cbor_major_type_text_string
 
-val cbor_nondet_mk_tagged (_: unit) : mk_tagged_t #_ cbor_nondet_match
+val cbor_nondet_mk_tagged (_: unit) : mk_tagged_safe_t #_ cbor_nondet_match
 
 val cbor_nondet_mk_array (_: unit) : mk_array_from_arrayptr_t #_ cbor_nondet_match
 
 val cbor_nondet_mk_map_entry (_: unit) : mk_map_entry_t #_ #_ cbor_nondet_match cbor_nondet_map_entry_match
 
-val cbor_nondet_mk_map_gen (_: unit)
+val cbor_nondet_mk_map (_: unit)
 : mk_map_from_arrayptr_safe_t #cbor_nondet_t #cbor_nondet_map_entry_t cbor_nondet_match cbor_nondet_map_entry_match
